Calculate powers of two quicker by using the equivalent of a linear shift rather than actual multiplications.  On my machine   EVAL ``2 ** 400`` now takes .12s rather than 9.7s.  I think comparable improvements should be possible for multiplications by powers of two.  Note that I'm relying on the fact that computeLib gives precedence to later patterns over earlier ones when it finds a rule to apply.

src/num/reduce/src/reduceLib.sml
@@ -36,7 +36,8 @@ val numeral_redns =
       numeral_iisuc, numeral_add, numeral_mult, iDUB_removal,
       numeral_sub, numeral_lt, numeral_lte, iSUB_THM,
       numeral_exp, numeral_evenodd, iSQR, numeral_fact,numeral_funpow,
-      numeral_MAX, numeral_MIN, numeral_div2, MOD_2EXP, numeral_imod_2exp];
+      numeral_MAX, numeral_MIN, numeral_div2, MOD_2EXP, numeral_imod_2exp,
+      TWO_EXP_THM, numeral_texp_help];
 
 val div_thm =
     prove
